end of day 27/03/20

inference-tool/src/main/scala/inference/Config.scala
@@ -49,10 +49,10 @@ case class Config(
 object Config {
   val builder = OParser.builder[Config]
   var config: Config = null
-  var heuristics = Inference.try_heuristics(List(), (Inference.nondeterministic_pairs _))
+  var heuristics = (Inference.null_modifier _).curried
   var numStates: BigInt = 0
   var ptaNumStates: BigInt = 0
-  var preprocessor: FSet.fset[(List[Nat.nat], ((Nat.nat, Nat.nat), Transition.transition_ext[Unit]))] => (List[List[(String, (List[Value.value], List[Value.value]))]] => ((List[Nat.nat] => (List[Nat.nat] => (Nat.nat => (FSet.fset[(List[Nat.nat], ((Nat.nat, Nat.nat), Transition.transition_ext[Unit]))] => (FSet.fset[(List[Nat.nat], ((Nat.nat, Nat.nat), Transition.transition_ext[Unit]))] => (FSet.fset[(List[Nat.nat], ((Nat.nat, Nat.nat), Transition.transition_ext[Unit]))] => ((FSet.fset[(List[Nat.nat], ((Nat.nat, Nat.nat), Transition.transition_ext[Unit]))] => FSet.fset[(Nat.nat, ((Nat.nat, Nat.nat), ((Transition.transition_ext[Unit], List[Nat.nat]), (Transition.transition_ext[Unit], List[Nat.nat]))))]) => Option[FSet.fset[(List[Nat.nat], ((Nat.nat, Nat.nat), Transition.transition_ext[Unit]))]]))))))) => ((FSet.fset[(List[Nat.nat], ((Nat.nat, Nat.nat), Transition.transition_ext[Unit]))] => FSet.fset[(Nat.nat, ((Nat.nat, Nat.nat), ((Transition.transition_ext[Unit], List[Nat.nat]), (Transition.transition_ext[Unit], List[Nat.nat]))))]) => FSet.fset[(List[Nat.nat], ((Nat.nat, Nat.nat), Transition.transition_ext[Unit]))]))) = null
+  var preprocessor: FSet.fset[(List[Nat.nat], ((Nat.nat, Nat.nat), Transition.transition_ext[Unit]))] => (List[List[(String, (List[Value.value], List[Value.value]))]] => ((Set.set[(Nat.nat, Nat.nat)] => (List[Nat.nat] => (List[Nat.nat] => (Nat.nat => (FSet.fset[(List[Nat.nat], ((Nat.nat, Nat.nat), Transition.transition_ext[Unit]))] => (FSet.fset[(List[Nat.nat], ((Nat.nat, Nat.nat), Transition.transition_ext[Unit]))] => (FSet.fset[(List[Nat.nat], ((Nat.nat, Nat.nat), Transition.transition_ext[Unit]))] => ((FSet.fset[(List[Nat.nat], ((Nat.nat, Nat.nat), Transition.transition_ext[Unit]))] => FSet.fset[(Nat.nat, ((Nat.nat, Nat.nat), ((Transition.transition_ext[Unit], List[Nat.nat]), (Transition.transition_ext[Unit], List[Nat.nat]))))]) => (Option[FSet.fset[(List[Nat.nat], ((Nat.nat, Nat.nat), Transition.transition_ext[Unit]))]], Set.set[(Nat.nat, Nat.nat)]))))))))) => ((FSet.fset[(List[Nat.nat], ((Nat.nat, Nat.nat), Transition.transition_ext[Unit]))] => FSet.fset[(Nat.nat, ((Nat.nat, Nat.nat), ((Transition.transition_ext[Unit], List[Nat.nat]), (Transition.transition_ext[Unit], List[Nat.nat]))))]) => FSet.fset[(List[Nat.nat], ((Nat.nat, Nat.nat), Transition.transition_ext[Unit]))]))) = null
 
   implicit val heuristicsRead: scopt.Read[Heuristics.Value] = scopt.Read.reads(Heuristics withName _)
   implicit val proprocessorsRead: scopt.Read[Preprocessors.Value] = scopt.Read.reads(Preprocessors withName _)
@@ -188,8 +188,8 @@ object Config {
 
         // Set up the heuristics
         val heuristics = scala.collection.immutable.Map(
-          Heuristics.store -> Store_Reuse.heuristic_1(config.train),
-          Heuristics.inputgen -> Store_Reuse.heuristic_2(config.train),
+          Heuristics.store -> (Store_Reuse.heuristic_1 _).curried(config.train),
+          Heuristics.inputgen -> (Store_Reuse.heuristic_2 _).curried(config.train),
           Heuristics.inc -> (Increment_Reset.insert_increment_2 _).curried,
           Heuristics.distinguish -> (Distinguishing_Guards.distinguish _).curried(config.train),
           Heuristics.same -> (Same_Register.same_register _).curried,
