inference-tool/src/main/scala/inference/Log.scala
@@ -8,8 +8,10 @@ object Log {
   val root =  LoggerFactory.getLogger("root").asInstanceOf[Logger]
   root.setLevel(Config.config.logLevel)
 
-  def logStates(s_1: Nat.nat, s_2: Nat.nat) = {
+  def logStates(e: Types.IEFSM, s_2: Nat.nat) = {
+		val s_1 = FSet.size_fset(Inference.S(e))
 		Config.numStates = Code_Numeral.integer_of_nat(s_1)
+		PrettyPrinter.iEFSM2dot(e, f"${PrettyPrinter.show(s_1)}-${PrettyPrinter.show(s_2)}")
 		// println(Config.numStates)
     root.debug(s"${Code_Numeral.integer_of_nat(s_2)} -> ${Code_Numeral.integer_of_nat(s_1)}")
   }
