formal/inference/heuristics/Weak_Subsumption.thy
@@ -6,7 +6,7 @@ definition maxBy :: "('a \<Rightarrow> 'b::linorder) \<Rightarrow> 'a \<Rightarr
   "maxBy f a b = (if (f a > f b) then a else b)"
 
 fun weak_subsumption :: "log \<Rightarrow> update_modifier" where
-  "weak_subsumption log t1ID t2ID s new _ old _ = (let
+  "weak_subsumption log closed t1ID t2ID s new _ old _ = (let
      t1 = get_by_ids new t1ID;
      t2 = get_by_ids new t2ID
      in
@@ -19,17 +19,17 @@ fun weak_subsumption :: "log \<Rightarrow> update_modifier" where
         newEFSMmax = replace_all new [t1ID, t2ID] maxT in
       \<comment> \<open>Most of the time, we'll want the transition with the most updates so start with that one\<close>
       if satisfies (set log) (tm newEFSMmax) then
-        Some newEFSMmax
+        (Some newEFSMmax, closed)
       else
         \<comment> \<open>There may be other occasions where we want to try the other transition\<close>
         \<comment> \<open>e.g. if their updates are equal but one has a different guard\<close>
         let newEFSMmin = replace_all new [t1ID, t2ID] minT in
         if satisfies (set log) (tm newEFSMmin) then
-          Some newEFSMmin
+          (Some newEFSMmin, closed)
         else
-          None
+          (None, closed)
      else
-      None
+      (None, closed)
    )"
 
 end
